theories/channel/multi_proto_consistency_examples.v
@@ -1,0 +1,293 @@
+From iris.algebra Require Import gmap excl_auth gmap_view.
+From iris.proofmode Require Import proofmode.
+From iris.base_logic Require Export lib.iprop.
+From iris.base_logic Require Import lib.own.
+From iris.program_logic Require Import language.
+From actris.channel Require Import multi_proto_model multi_proto.
+Set Default Proof Using "Type".
+Export action.
+
+Definition iProto_example1 {Σ V} : gmap nat (iProto Σ V) :=
+  ∅.
+
+Lemma iProto_example1_consistent {Σ V} :
+  ⊢ iProto_consistent (@iProto_example1 Σ V).
+Proof.
+  rewrite iProto_consistent_unfold.
+  iIntros (i j m1 m2) "Hi Hj".
+  rewrite lookup_total_empty.
+  by rewrite iProto_end_message_equivI.
+Qed.
+
+Definition iProto_example2 `{!invGS Σ} (P : iProp Σ) : gmap nat (iProto Σ Z) :=
+  <[0 := (<(Send 1) @ (x:Z)> MSG x {{ P }} ; END)%proto ]>
+  (<[1 := (<(Recv 0) @ (x:Z)> MSG x {{ P }} ; END)%proto ]>
+   ∅).
+
+Lemma iProto_example2_consistent `{!invGS Σ} (P : iProp Σ) :
+  ⊢ iProto_consistent (@iProto_example2 _ Σ invGS0 P).
+Proof.
+  rewrite iProto_consistent_unfold.
+  rewrite /iProto_example2.
+  iIntros (i j m1 m2) "Hm1 Hm2".
+  destruct i, j.
+  - rewrite !lookup_total_insert.
+    rewrite !iProto_message_equivI.
+    iDestruct "Hm1" as (Hieq) "#Hm1".
+    iDestruct "Hm2" as (Hjeq) "#Hm2".
+    done.
+  - destruct j; last first.
+    { rewrite !lookup_total_insert.
+      rewrite !iProto_message_equivI.
+      iDestruct "Hm1" as (Hieq) "#Hm1". done. }
+    rewrite !lookup_total_insert.
+    rewrite lookup_total_insert_ne; [|done].
+    rewrite !lookup_total_insert.
+    rewrite !iProto_message_equivI.
+    iDestruct "Hm1" as (Hieq) "#Hm1".
+    iDestruct "Hm2" as (Hjeq) "#Hm2".
+    iIntros (v p1) "Hm1'".
+    iSpecialize ("Hm1" $!v (Next p1)).
+    rewrite iMsg_base_eq. simpl.
+    rewrite iMsg_exist_eq. simpl.
+    iRewrite -"Hm1" in "Hm1'".
+    iExists END%proto.
+    iSpecialize ("Hm2" $!v (Next END%proto)).
+    iRewrite -"Hm2".
+    simpl.
+    iDestruct "Hm1'" as (x Heq) "[#Heq HP]".
+    iSplitL.
+    { iExists x. iSplit; [done|]. iFrame. done. }
+    iNext. iRewrite -"Heq".
+    rewrite insert_commute; [|done].
+    rewrite insert_insert.
+    rewrite insert_commute; [|done].
+    rewrite insert_insert.
+    rewrite iProto_consistent_unfold.
+    iIntros (i' j' m1' m2') "Hm1' Hm2'".
+    destruct i'.
+    { rewrite lookup_total_insert.
+      iDestruct (iProto_end_message_equivI with "Hm1'") as "H".
+      done. }
+    destruct i'.
+    { rewrite lookup_total_insert_ne; [|done].
+      rewrite lookup_total_insert.
+      iDestruct (iProto_end_message_equivI with "Hm1'") as "H".
+      done. }
+    rewrite lookup_total_insert_ne; [|done].
+    rewrite lookup_total_insert_ne; [|done].
+    rewrite lookup_total_alt. simpl.
+    iDestruct (iProto_end_message_equivI with "Hm1'") as "H".
+    done.
+  - destruct i; last first.
+    { rewrite lookup_total_insert_ne; [|done].
+      rewrite lookup_total_insert_ne; [|done].
+      rewrite lookup_total_alt. simpl.
+      iDestruct (iProto_end_message_equivI with "Hm1") as "H".
+      done. }
+    rewrite !lookup_total_insert.
+    rewrite lookup_total_insert_ne; [|done].
+    rewrite !lookup_total_insert.
+    rewrite !iProto_message_equivI.
+    iDestruct "Hm1" as (Hieq) "#Hm1". done.
+  - destruct i.
+    { rewrite lookup_total_insert_ne; [|done].
+      rewrite lookup_total_insert.
+      rewrite !iProto_message_equivI.
+      iDestruct "Hm1" as (Hieq) "#Hm1". done. }
+    rewrite lookup_total_insert_ne; [|done].
+    rewrite lookup_total_insert_ne; [|done].
+    rewrite lookup_total_alt. simpl.
+    iDestruct (iProto_end_message_equivI with "Hm1") as "H".
+    done.
+Qed.
+
+Definition iProto_example3 `{!invGS Σ}  : gmap nat (iProto Σ Z) :=
+  <[0 := (<(Send 1) @ (x:Z)> MSG x ; <(Recv 2)> MSG x; END)%proto ]>
+  (<[1 := (<(Recv 0) @ (x:Z)> MSG x ; <(Send 2)> MSG x; END)%proto ]>
+  (<[2 := (<(Recv 1) @ (x:Z)> MSG x ; <(Send 0)> MSG x; END)%proto ]>
+    ∅)).
+
+Lemma iProto_example3_consistent `{!invGS Σ} :
+  ⊢ iProto_consistent (@iProto_example3 _ Σ invGS0).
+Proof.
+  rewrite iProto_consistent_unfold.
+  rewrite /iProto_example3.
+  iIntros (i j m1 m2) "Hm1 Hm2".
+  destruct i; last first.
+  { destruct i.
+    { rewrite lookup_total_insert_ne; [|done].
+      rewrite !lookup_total_insert.
+      rewrite !iProto_message_equivI.
+      by iDestruct "Hm1" as (Hieq) "#Hm1". }
+    destruct i.
+    { rewrite lookup_total_insert_ne; [|done].
+      rewrite lookup_total_insert_ne; [|done].
+      rewrite !iProto_message_equivI.
+      by iDestruct "Hm1" as (Hieq) "#Hm1". }
+    rewrite lookup_total_insert_ne; [|done].
+    rewrite lookup_total_insert_ne; [|done].
+    rewrite lookup_total_insert_ne; [|done].
+    rewrite lookup_total_empty=> /=.
+    by rewrite iProto_end_message_equivI. }
+  destruct j.
+  { rewrite !lookup_total_insert.
+    rewrite !iProto_message_equivI.
+    by iDestruct "Hm2" as (Hjeq) "#Hm2". }
+  destruct j; last first.
+  { rewrite !lookup_total_insert.
+    rewrite lookup_total_insert_ne; [|done].
+    rewrite lookup_total_insert_ne; [|done].
+    destruct j.
+    { rewrite !lookup_total_insert.
+      rewrite !iProto_message_equivI.
+      by iDestruct "Hm2" as (Hjeq) "#Hm2". }
+    rewrite lookup_total_insert_ne; [|done].
+    rewrite lookup_total_empty=> /=.
+    by rewrite iProto_end_message_equivI. }
+  rewrite !lookup_total_insert.
+  rewrite lookup_total_insert_ne; [|done].
+  rewrite !lookup_total_insert.
+  rewrite !iProto_message_equivI.
+  iDestruct "Hm1" as (Hieq) "#Hm1".
+  iDestruct "Hm2" as (Hjeq) "#Hm2".
+  iIntros (v p1) "Hm1'".
+  iSpecialize ("Hm1" $!v (Next p1)).
+  rewrite !iMsg_base_eq.
+  rewrite !iMsg_exist_eq.
+  iRewrite -"Hm1" in "Hm1'".
+  iDestruct "Hm1'" as (x Heq) "[#Hm1' _]".
+  iSpecialize ("Hm2" $!v (Next (<Send 2> iMsg_base_def x True END)))%proto.
+  iExists (<Send 2> iMsg_base_def x True END)%proto.
+  iRewrite -"Hm2".
+  simpl.
+  iSplitL.
+  { iExists x. iSplit; [done|]. iFrame. done. }
+  iNext.
+  rewrite iProto_consistent_unfold.
+  rewrite insert_commute; [|done].
+  rewrite insert_insert.
+  rewrite insert_commute; [|done].
+  rewrite insert_insert.
+  iRewrite -"Hm1'".
+  iClear (m1 m2 Hieq Hjeq p1 v Heq) "Hm1 Hm2 Hm1'".
+  iIntros (i j m1 m2) "Hm1 Hm2".
+  destruct i.
+  { rewrite !lookup_total_insert.
+    rewrite !iProto_message_equivI.
+    by iDestruct "Hm1" as (Hieq) "#Hm1". }
+  rewrite lookup_total_insert_ne; [|done].
+  destruct i; last first.
+  { destruct i.
+    { rewrite lookup_total_insert_ne; [|done].
+      rewrite lookup_total_insert.
+      rewrite !iProto_message_equivI.
+      by iDestruct "Hm1" as (Hieq) "#Hm1". }
+    rewrite lookup_total_insert_ne; [|done].
+    rewrite lookup_total_insert_ne; [|done].
+    rewrite lookup_total_empty=> /=.
+    by rewrite iProto_end_message_equivI. }
+  rewrite lookup_total_insert.
+  destruct j.
+  { rewrite lookup_total_insert.
+    rewrite !iProto_message_equivI.
+    by iDestruct "Hm2" as (Hjeq) "#Hm2". }
+  rewrite lookup_total_insert_ne; [|done].
+  destruct j.
+  { rewrite lookup_total_insert.
+    rewrite !iProto_message_equivI.
+    by iDestruct "Hm2" as (Hjeq) "#Hm2". }
+  rewrite lookup_total_insert_ne; [|done].
+  destruct j; last first.
+  { rewrite lookup_total_insert_ne; [|done].
+    rewrite lookup_total_empty.
+    by rewrite iProto_end_message_equivI. }
+  rewrite lookup_total_insert.
+  rewrite !iProto_message_equivI.
+  iDestruct "Hm1" as (Hieq) "#Hm1".
+  iDestruct "Hm2" as (Hjeq) "#Hm2".
+  iIntros (v p1) "Hm1'".
+  iSpecialize ("Hm1" $!v (Next p1)).
+  iRewrite -"Hm1" in "Hm1'".
+  iDestruct "Hm1'" as (Heq) "[#Hm1' _]".
+  iSpecialize ("Hm2" $!v (Next (<Send 0> iMsg_base_def x True END)))%proto.
+  iExists (<Send 0> iMsg_base_def x True END)%proto.
+  iRewrite -"Hm2".
+  simpl.
+  iSplitL.
+  { iExists x. iSplit; [done|]. iFrame. done. }
+  iNext.
+  rewrite iProto_consistent_unfold.
+  rewrite (insert_commute _ 1 2); [|done].
+  rewrite (insert_commute _ 1 0); [|done].
+  rewrite insert_insert.
+  rewrite (insert_commute _ 2 0); [|done].
+  rewrite (insert_commute _ 2 1); [|done].
+  rewrite insert_insert.
+  iRewrite -"Hm1'".
+  iClear (m1 m2 Hieq Hjeq p1 v Heq) "Hm1 Hm2 Hm1'".
+  iIntros (i j m1 m2) "Hm1 Hm2".
+  destruct i.
+  { rewrite !lookup_total_insert.
+    rewrite !iProto_message_equivI.
+    by iDestruct "Hm1" as (Hieq) "#Hm1". }
+  rewrite lookup_total_insert_ne; [|done].
+  destruct i.
+  { rewrite lookup_total_insert.
+    by rewrite iProto_end_message_equivI. }
+  rewrite lookup_total_insert_ne; [|done].
+  destruct i; last first.
+  { rewrite lookup_total_insert_ne; [|done].
+    rewrite lookup_total_empty.
+    by rewrite iProto_end_message_equivI. }
+  rewrite lookup_total_insert.
+  destruct j; last first.
+  { rewrite lookup_total_insert_ne; [|done].
+    destruct j.
+    { rewrite lookup_total_insert.
+      by rewrite iProto_end_message_equivI. }
+    rewrite lookup_total_insert_ne; [|done].
+    destruct j.
+    { rewrite lookup_total_insert.
+      rewrite !iProto_message_equivI.
+      by iDestruct "Hm2" as (Hjeq) "#Hm2". }
+    rewrite lookup_total_insert_ne; [|done].
+    rewrite lookup_total_empty.
+    by rewrite iProto_end_message_equivI. }
+  rewrite lookup_total_insert.
+  rewrite !iProto_message_equivI.
+  iDestruct "Hm1" as (Hieq) "#Hm1".
+  iDestruct "Hm2" as (Hjeq) "#Hm2".
+  iIntros (v p1) "Hm1'".
+  iSpecialize ("Hm1" $!v (Next p1)).
+  iRewrite -"Hm1" in "Hm1'".
+  iDestruct "Hm1'" as (Heq) "[#Hm1' _]".
+  iSpecialize ("Hm2" $!v (Next END))%proto.
+  iExists END%proto.
+  iRewrite -"Hm2".
+  simpl.
+  iSplitL; [done|].
+  rewrite insert_insert.
+  rewrite insert_commute; [|done].
+  rewrite (insert_commute _ 2 1); [|done].
+  rewrite insert_insert.
+  iNext.
+  iRewrite -"Hm1'".
+  rewrite iProto_consistent_unfold.
+  iClear (m1 m2 Hieq Hjeq p1 v Heq) "Hm1 Hm2 Hm1'".
+  iIntros (i j m1 m2) "Hm1 Hm2".
+  destruct i.
+  { rewrite lookup_total_insert.
+    by rewrite !iProto_end_message_equivI. }
+  rewrite lookup_total_insert_ne; [|done].
+  destruct i.
+  { rewrite lookup_total_insert.
+    by rewrite !iProto_end_message_equivI. }
+  rewrite lookup_total_insert_ne; [|done].
+  destruct i.
+  { rewrite lookup_total_insert.
+    by rewrite !iProto_end_message_equivI. }
+  rewrite lookup_total_insert_ne; [|done].
+  rewrite lookup_total_empty.
+  by rewrite iProto_end_message_equivI.
+Qed.
